```python
n, m, k = map(int, input().split())
li = list(map(int, input().split()))

li.sort()

first = li[-1]
second = li[-2]

count_of_first = m - (m // k)
count_of_second = m // k

result = first * count_of_first + second * count_of_second
print(result)
```

공책에 써보면서 법칙을 찾아냈다
| m   | k   | count_of_first | count_of_second |
| --- | --- | ----- | ------ |
| 4   | 3   | 3     | 1      |
| 5   | 3   | 4     | 1      |
| 6   | 3   | 5     | 1      |
| 7   | 3   | 6     | 1      |
| 8   | 3   | 6     | 2      |
| 9   | 3   | 7     | 2      |
| 10  | 3   | 8     | 2      |
| 11  | 3   | 9     | 2      |
| 12  | 3   | 9     | 3       |

우선 `m = count_of_first + count_of_second` 임을 찾아냈고
그 다음으로는 `count_of_second = m // k` 임을 찾아냈다.







